\documentclass[12pt]{article}

\addtolength{\textwidth}{.6in}
\addtolength{\oddsidemargin}{-.3in}
\setlength{\textheight}{8.4in}
\setlength{\topmargin}{-.25in}
\setlength{\headheight}{0.0in}
\renewcommand{\baselinestretch}{1.0}
\linespread{1.15}

\usepackage{cite}
\usepackage{times, verbatim,xcolor,bm}
\usepackage{amsbsy,amssymb, amsmath, amsthm}
\usepackage{hyperref}

\newtheorem{definition}{Definition}
\newtheorem{theorem}{Theorem}
\newtheorem{lemma}{Lemma}
\newtheorem{corollary}{Corollary}
\newtheorem{assumption}{Assumption}
\newtheorem{fact}{Fact}

\newcommand{\ve}{\varepsilon}
\newcommand{\ov}{\overline}
\newcommand{\un}{\underline}
\newcommand{\ta}{\theta}
\newcommand{\Ta}{\Theta}
\newcommand{\expect}{\mathbb{E}}

\begin{document}
\title{\vskip-0.6in Gradualism}
\author{ECN 490}
\date{\today}
\maketitle


\section{Original Model with Government / Lobbying Effort}
\title{Lobby}
\[
\max_{e^t,m^t,l^t} \sum_{t=1}^\infty \beta^{t-1}\left\{A(m_t)F^\alpha\cdot l^{1-\alpha}_t\left[P^W+\tau(\gamma(e_{t-1}))\right]-l_t-\mu_t-e_t
  \right\} \hskip.2in \text{s.t.} \hskip.2in  m_t=m_{t-1}+\mu_t
\]

 
\title{Bellman Equation}
\[
  V_l(e_t,m_t)=\max_{e_t,m_t,l_t}\left\{A(m_t)F^\alpha\cdot (l_t)^{1-\alpha}\left[P^W+\tau(\gamma(e_{t-1}))\right]-l_t-\mu_t-e_t+\beta V_l(e_{t+1},m_{m+t}
  \right\} \hskip.2in 
\]
\title{Value Function}
\[
  V_l(e_t^\ast,m_t^\ast)=\left\{A(m_t^\ast)F^\alpha\cdot (l^\ast_t)^{1-\alpha}\left[P^W+\tau(\gamma(e_{t-1}^\ast))\right]-l_t^\ast-\mu_t^\ast-e_t^\ast+\beta V_l(e^\ast_{t+1},m^\ast_{t+1})
  \right\} \hskip.2in
\]

\[
t=\text{this period}
\]
\[
t+1=\text{next period}
\]
\[
\beta=\text{discount factor}
\]
\[
l=\text{lobby}
\]

\section{No Government / Lobbying Effort}
\title{Lobby}
\[
\max_{m^t,l^t} \sum_{t=1}^\infty \beta^{t-1}\left\{A(m_t)F^\alpha\cdot l^{1-\alpha}_t\cdot P^W-l_t-\mu_t
  \right\} \hskip.2in \text{s.t.} \hskip.2in  m_t=m_{t-1}+\mu_t
\]

 
\title{Bellman Equation}
\[
  V_l(m_t)=\max_{m_t,l_t}\left\{A(m_t)F^\alpha\cdot (l_t)^{1-\alpha}\cdot P^W-l_t-(m_t-m_{t-1})+\beta V_l(m_{t+1})
  \right\} \hskip.2in 
\]
\title{Value Function}
\[
  V_l(e_t^\ast,m_t^\ast)=\left\{A(m_t^\ast)F^\alpha\cdot (l^\ast_t)^{1-\alpha}\cdot P^W-l_t^\ast-(m^\ast_t-m_{t-1})+\beta V_l(m^\ast_{t+1})
  \right\} \hskip.2in
\]
\title{FOCs}
\[\dfrac{\delta V_L}{\delta m_t^\ast}=\dfrac{\delta A}{\delta m^\ast_t} \cdot F^\alpha \cdot l^{1-\alpha}_t \cdot P^W +\beta [\dfrac{\delta V_L(m_{t+1^\ast})}{\delta(m_{t+1^\ast})} \cdot 1] =1
\hskip.2in
\]
\[
\dfrac{\delta V_L}{\delta \mu_t}=\dfrac{d^A}{dM_t} \cdot \dfrac{dM_t}{d\mu_t} \cdot F^\alpha \cdot l_t^{1-\alpha} \cdot P^W + \beta[\dfrac{\delta V_L(m_{t+1})}{\delta(m_{t+1})} \cdot 1] =1
\hskip.2in 
\]
\[
\dfrac{\delta V_L}{\delta l_t}= (1-\alpha) A(m_{t-1}+\mu_t) \cdot F^\alpha \cdot 1^{-\alpha} \cdot P^W =1
\hskip.2in 
\]
\[
\dfrac{\dfrac{\delta A}{\delta m_t} \cdot l^t}{(1-\alpha) A(m_{t+1}+\mu_t)} +\beta \dfrac{\delta V_L (m_{t+1})}{\delta m_{t+1}} =1
\hskip.2in
\]
\[
t=\text{this period}
\]
\[
t+1=\text{next period}
\]
\[
\beta=\text{discount factor}
\]
\[
l=\text{lobby}
\]
note: 1 comes from $\dfrac{\delta m_{t+1}}{\delta \mu}$
\end{document}